Use `notypeclasses refine` in `iPoseProof` helpers.
Also, rewrite `iIntoEmpValid`. Now, instead of using Ltac to traverse
the type of the term and generate goals for the premises, we repeatedly
apply a series of lemmas. This has the advantage that it works up to
convertability, and we no longer need the `eval ...` hacks.

theories/proofmode/coq_tactics.v
@@ -452,8 +452,19 @@ Proof.
   by rewrite -(entails_wand P) // intuitionistically_emp emp_wand.
 Qed.
 
-Lemma tac_pose_proof Δ j P Q :
-  P →
+Definition IntoEmpValid (φ : Type) (P : PROP) := φ → bi_emp_valid P.
+Lemma into_emp_valid_here φ P : AsEmpValid φ P → IntoEmpValid φ P.
+Proof. by intros [??]. Qed.
+Lemma into_emp_valid_impl (φ ψ : Type) P :
+  φ → IntoEmpValid ψ P → IntoEmpValid (φ → ψ) P.
+Proof. rewrite /IntoEmpValid; auto. Qed.
+Lemma into_emp_valid_forall {A} (φ : A → Type) P x :
+  IntoEmpValid (φ x) P → IntoEmpValid (∀ x : A, φ x) P.
+Proof. rewrite /IntoEmpValid; auto. Qed.
+
+Lemma tac_pose_proof Δ j (φ : Prop) P Q :
+  φ →
+  IntoEmpValid φ P →
   match envs_app true (Esnoc Enil j P) Δ with
   | None => False
   | Some Δ' => envs_entails Δ' Q
@@ -461,8 +472,8 @@ Lemma tac_pose_proof Δ j P Q :
   envs_entails Δ Q.
 Proof.
   destruct (envs_app _ _ _) as [Δ'|] eqn:?; last done.
-  rewrite envs_entails_eq => HP ?. rewrite envs_app_singleton_sound //=.
-  by rewrite -HP /= intuitionistically_emp emp_wand.
+  rewrite envs_entails_eq => ? HP <-. rewrite envs_app_singleton_sound //=.
+  by rewrite -HP //= intuitionistically_emp emp_wand.
 Qed.
 
 Lemma tac_pose_proof_hyp Δ i j Q :
